benchmark/task9/Filesystem.dfy
@@ -64,14 +64,14 @@ module {:options "-functionSyntax:4"} Filesystem {
     // method Open(file: string, perm: Permission) returns (res: Result<object, string>)
     method Open(file: string) returns (res: Result<object, string>)
       modifies this
-      ensures res.Success? ==> is_open == (file != "~/.ssh/id_rsa.txt") 
+      ensures res.Success? ==> is_open == !Utils.access_to_private_key(file)
     {
       var isError, fileStream, errorMsg := INTERNAL_Open(file);
       var privateKeyAccess := true;
       if (|file| >= 4) {
-        privateKeyAccess := file[0..4] == "~/.ssh/id_rsa.txt";
+        privateKeyAccess := Utils.access_to_private_key(file);
       }
-      is_open := (file != "~/.ssh/id_rsa.txt");
+      is_open := !Utils.access_to_private_key(file);
       return if (isError || privateKeyAccess) then Failure(errorMsg) else Success(fileStream);
     }
 
